Basic API with add, find, remove, clear and free

kremlib/LowStar.Lib.AssocList.fst
@@ -18,6 +18,9 @@ open LowStar.BufferOps
 
 #set-options "--fuel 0 --ifuel 0"
 
+/// Types, invariants, footprint
+/// ----------------------------
+
 /// We prefer the packed representation that is in general easier to use and will
 /// look at the underlying predicate-based representation from LL1 only when
 /// strictly needed.
@@ -34,7 +37,7 @@ let map k v =
 
 /// Functions suffixed with an underscore operate on either LL1 or raw lists
 /// while those without operate on LL2.
-val v_: #t_k:eqtype -> #t_v:Type0 -> l:list (t_k & t_v) -> GTot (map t_k t_v)
+val v_: #t_k:eqtype -> #t_v:Type0 -> l:list (t_k & t_v) -> Tot (map t_k t_v)
 let v_ #_ #t_v l =
   List.Tot.fold_right (fun (k, v) m -> M.upd m k (Some v)) l (M.const (None #t_v))
 
@@ -58,7 +61,12 @@ let footprint #_ #_ h ll =
 ///
 /// B.(loc_disjoint l (loc_all_regions_from true r)) ==> B.(loc_disjoint l (footprint h ll))
 ///
-/// This would allow clients to deduce that their own allocations are disjoint from the footprint of this. And also to apply the framing lemma with proper patterns!
+/// This would allow clients to deduce that their own allocations are disjoint
+/// from the footprint of this. And also to apply the framing lemma with proper
+/// patterns!
+
+/// Find
+/// ----
 
 /// Proper recursion can only be done over the LL1.t type (unpacked representation).
 val find_ (#t_k: eqtype) (#t_v: Type0) (hd: LL1.t (t_k & t_v)) (l: G.erased (list (t_k & t_v))) (k: t_k):
@@ -83,8 +91,6 @@ let rec find_ #_ #_ hd l k =
       find_ cell.LL1.next (List.Tot.tl l) k
 #pop-options
 
-/// A wrapper for LL2
-
 val find (#t_k: eqtype) (#t_v: Type0) (ll: t t_k t_v) (k: t_k):
   Stack (option t_v)
     (requires fun h0 ->
@@ -97,15 +103,140 @@ val find (#t_k: eqtype) (#t_v: Type0) (ll: t t_k t_v) (k: t_k):
 let find #_ #_ ll k =
   find_ !*ll.LL2.ptr !*ll.LL2.v k
 
+/// Adding elements
+/// ---------------
+
 val add (#t_k: eqtype) (#t_v: Type0) (ll: t t_k t_v) (k: t_k) (x: t_v):
   ST unit
     (requires fun h0 ->
       invariant h0 ll)
     (ensures fun h0 _ h1 ->
       B.modifies (footprint h0 ll) h0 h1 /\
+      invariant h1 ll /\
       v h1 ll == M.upd (v h0 ll) k (Some x))
 
 #push-options "--fuel 1"
 let add #_ #_ ll k x =
   LL2.push ll (k, x)
 #pop-options
+
+/// Removing elements
+/// -----------------
+
+/// This one is tricky to state so temporarily disabled. I'm trying to offer a
+/// shadowing API that allows revealing the previous binding (if any) when the
+/// most recent one is remoed. However, as it stands, the precondition is not
+/// strong enough to conclude that just popping the first occurrence of key
+/// ``k`` in the list yields ``m``.
+///
+/// I'm unsure on how to do that cleanly and abstractly without revealing to the
+/// client the underlying associative-list nature of the map abstraction, so
+/// disabling for now.
+///
+(*val remove_one (#t_k: eqtype)
+  (#t_v: Type0)
+  (ll: t t_k t_v)
+  (k: t_k)
+  (x: G.erased t_v)
+  (m: G.erased (map t_k t_v)):
+  ST unit
+    (requires fun h0 ->
+      invariant h0 ll /\
+      // TODO: file bug to figure why auto-reveal doesn't work (also in post-condition)
+      v h0 ll == M.upd m k (Some (G.reveal x)))
+    (ensures fun h0 _ h1 ->
+      B.modifies (footprint h0 ll) h0 h1 /\
+      v h1 ll == G.reveal m)*)
+
+val remove_all_ (#t_k: eqtype) (#t_v: Type0) (hd: LL1.t (t_k & t_v)) (l: G.erased (list (t_k & t_v))) (k: t_k):
+  ST (LL1.t (t_k & t_v) & G.erased (list (t_k & t_v)))
+    (requires fun h0 ->
+      LL1.well_formed h0 hd l /\
+      LL1.invariant h0 hd l)
+    (ensures fun h0 (hd', l') h1 ->
+      LL1.well_formed h1 hd' l' /\
+      LL1.invariant h1 hd' l' /\
+      B.(loc_includes (LL1.footprint h0 hd l) (LL1.footprint h1 hd' l')) /\
+      B.modifies (LL1.footprint h0 hd l) h0 h1 /\
+      v_ l' == M.upd (v_ l) k None)
+
+#push-options "--fuel 1 --ifuel 1 --z3rlimit 50"
+let rec remove_all_ #t_k #t_v hd l k =
+  let h0 = ST.get () in
+  if B.is_null hd then begin
+    M.lemma_equal_intro (v_ l) (M.upd (v_ l) k None);
+    hd, l
+  end else begin
+    let cell = !*hd in
+    let { LL1.data; LL1.next } = cell in
+    let k', v = data in
+    if k = k' then begin
+      B.free hd;
+      let h1 = ST.get () in
+      LL1.frame next (List.Tot.tail l) (B.loc_addr_of_buffer hd) h0 h1;
+      let hd', l' = remove_all_ next (List.Tot.tail l) k in
+      M.lemma_equal_intro (v_ l') (M.upd (v_ l) k None);
+      hd', l'
+    end else begin
+      let hd', l' = remove_all_ next (List.Tot.tail l) k in
+      hd *= { LL1.data; LL1.next = hd' };
+      let h1 = ST.get () in
+      M.lemma_equal_intro (v_ ((k', v) :: l')) (M.upd (v_ l) k None);
+      assert (LL1.well_formed h1 hd (data :: l'));
+      assert (LL1.invariant h1 hd (data :: l'));
+      hd, G.hide ((k', v) :: l')
+    end
+  end
+#pop-options
+
+val remove_all (#t_k: eqtype)
+  (#t_v: Type0)
+  (ll: t t_k t_v)
+  (k: t_k):
+  ST unit
+    (requires fun h0 ->
+      invariant h0 ll)
+    (ensures fun h0 _ h1 ->
+      B.modifies (footprint h0 ll) h0 h1 /\
+      invariant h1 ll /\
+      v h1 ll == M.upd (v h0 ll) k None)
+
+let remove_all #_ #_ ll k =
+  let open LL2 in
+  let hd, v = remove_all_ !*ll.ptr !*ll.v k in
+  ll.ptr *= hd;
+  ll.v *= v
+
+/// Clearing (resetting)
+/// --------------------
+
+val clear (#t_k: eqtype)
+  (#t_v: Type0)
+  (ll: t t_k t_v):
+  ST unit
+    (requires fun h0 ->
+      invariant h0 ll)
+    (ensures fun h0 _ h1 ->
+      B.modifies (footprint h0 ll) h0 h1 /\
+      invariant h1 ll /\
+      v h1 ll == M.const None)
+
+#push-options "--fuel 1"
+let clear #_ #_ ll =
+  LL2.clear ll
+#pop-options
+
+/// Freeing the resource
+/// --------------------
+
+val free (#t_k: eqtype)
+  (#t_v: Type0)
+  (ll: t t_k t_v):
+  ST unit
+    (requires fun h0 ->
+      invariant h0 ll)
+    (ensures fun h0 _ h1 ->
+      B.modifies (footprint h0 ll) h0 h1)
+
+let free #_ #_ ll =
+  LL2.free ll
